{
 "cells": [
  {
   "cell_type": "markdown",
   "metadata": {},
   "source": [
    "<h1 style=\"font-weight:Bold\">Discrete Structures 2 Programming Assignments</h1>\n"
   ]
  },
  {
   "cell_type": "markdown",
   "metadata": {},
   "source": [
    "Siobhan B. Leonor TTH 12:00 - 1:30PM"
   ]
  },
  {
   "cell_type": "markdown",
   "metadata": {},
   "source": [
    "**<h2>LECTURE 2:</h2>**\n"
   ]
  },
  {
   "cell_type": "markdown",
   "metadata": {},
   "source": [
    "**<h3>Task 1:</h3>**\n",
    "\n",
    "**<h4>Question 1:</h4>**\n",
    "\n",
    " Show that the expected value $E[y] = \\Sigma y \\cdotp P(y) = n \\cdot p_i$\n",
    "\n",
    "Step 1: Express the expected value $E[y]$ in terms of $P(y)$:\n",
    "\n",
    "- $E[y] = \\Sigma_{y} \\, y \\cdot P(y)$ \n",
    "\n",
    "Step 2: Substitute the given join probability distribution  for $P(y)$. \n",
    "\n",
    "- $E[y] = \\Sigma_{y} \\, y \\cdot (\\frac{n!}{y_1!y_2!y_3!...y_k!} \\cdot p_1^{y_1} p_2^{y_2} p_3^{y_3}....p_k^{y_k}) $ \n",
    "\n",
    "Step 3: Expand the sum:\n",
    "\n",
    "- $E[y] = \\Sigma_{y} \\frac{n!}{y_1!y_2!y_3!...y_k!} \\cdot (y_1 \\cdot p_1) \\cdot (y_2 \\cdot p_2) \\cdot (y_3 \\cdot p_3) \\ldots (y_k \\cdot p_k)$\n",
    "\n",
    "Step 4: Rearrange the terms:\n",
    "\n",
    "- $E[y] =  \\frac{n!}{y_1!y_2!y_3!...y_k!} \\cdot \\Sigma_{y} (y_1 \\cdot p_1) \\cdot (y_2 \\cdot p_2) \\cdot (y_3 \\cdot p_3) \\ldots (y_k \\cdot p_k)$\n",
    "\n",
    "Step 5: Observe that the sum is a product of sums:\n",
    "\n",
    "- $E[y] =  \\frac{n!}{y_1!y_2!y_3!...y_k!} \\cdot  ( \\Sigma_{y_1} \\,y_1 \\cdot p_1) \\cdot (\\Sigma_{y_2} \\, y_2 \\cdot p_2) \\cdot ( \\Sigma_{y_3} \\, y_3 \\cdot p_3) \\ldots ( \\Sigma_{y_k} \\, y_k \\cdot p_k)$\n",
    "\n",
    "Step 6: Each individual sum is simply th expected value of a binomial distribution with parameter $n$ and $p_i$:\n",
    "\n",
    "- $E[Y_i] = n \\cdot p_i$\n",
    "\n",
    "Step 7: Subsitute the expected values of each $Y_i$:\n",
    "\n",
    "- $E[y] = \\frac{n!}{y_1!y_2!y_3!...y_k!} \\cdot (n \\cdot p_1) \\cdot (n \\cdot p_2) \\cdot (n \\cdot p_3) \\ldots  (n \\cdot p_k)$\n",
    "\n",
    "Step 8: Notice that $n!$ and $y_1!y_2!y_3!...y_k!$ cancel out:\n",
    "\n",
    "- $E[y] = n \\cdot p_1 \\cdot n \\cdot p_2 \\cdot n \\cdot p_3 \\ldots n \\cdot p_k$\n",
    "\n",
    "We simplify the expression by combining terms and recognizing that the coeffcient $(y_1!y_2!y_3!...y_k!)$ can be simplified to $n!$, the number of permutations of outcomes.\n",
    "\n",
    "Step 9: Simplify\n",
    "\n",
    "- $E[y] = n  (p_1 \\cdot  p_2 \\cdot  p_3 \\ldots  p_k)$\n",
    "\n",
    "Step 10: Recall that $p_1 + p_2 + p_3 + \\ldots + p_k = 1 $\n",
    "\n",
    "- $E[y] = n \\cdot 1$\n",
    "- $E[y] = n \\cdot p_i$\n",
    "\n",
    "To conclude, the expected value  E[y] equals to $\\Sigma y \\cdotp P(y)$, which is equal to $n \\cdot p_i$ .\n"
   ]
  },
  {
   "cell_type": "markdown",
   "metadata": {},
   "source": [
    "$\\textbf{Question 2:}$\n",
    "\n",
    "Given:\n",
    "- $n = 500$ (total number of adults sampled)\n",
    "- $p_{65-100} = 0.16$ (probability of obtaining a person aged 65 and above)\n",
    "\n",
    "Step 1: Apply the Formula \n",
    "The expected value $E[Y_{65+}]$ is given by:\n",
    "\n",
    "- $ E[Y_{65+}] =  n \\cdot p_{65-100}$\n",
    "\n",
    "Step 2: Substitute Values\n",
    "\n",
    "- $ E[Y_{65+}] = 500 \\cdot 0.16$\n",
    "- $ E[Y_{65+}] = 80$\n",
    "\n",
    "Therefore, the expected value to obtain a person aged 65 and 100 is 80."
   ]
  },
  {
   "cell_type": "markdown",
   "metadata": {},
   "source": [
    "**<h3>Task 2:</h3>**"
   ]
  },
  {
   "cell_type": "markdown",
   "metadata": {},
   "source": [
    "**<h4>Question 1:</h4>**\n",
    "\n",
    "The probability distribution of $Y$ follows the binomial distribution, which can be calculated using the binomial probability mass function:\n",
    "\n",
    "- $P(Y = y) = \\binom{n}{y} \\cdot p^y \\cdot q^{n-y}$\n",
    "\n",
    "where:\n",
    "\n",
    "- $P(Y = y)$ is the probabiltiy of observing $y$ successes in $n$ trials.\n",
    "- $\\binom{n}{y}$ is the binomial coefficient , representing the number of ways to choose $y$ successes out of $n$ trials.\n",
    "- $p^y$ represents the probability of having $y$ successes.\n",
    "- $q^{n-y}$ represents the probability of having  $(n - y)$ failures.\n",
    "\n",
    "**<h4>Question 2:</h4>**\n",
    "\n",
    "Step 1: Define the Expectation\n",
    "\n",
    "- $E[y] = \\Sigma_{y = 0}^n \\cdot P(y)$.\n",
    "\n",
    "Step 2: Substitute the Binomial Probability Mass Function\n",
    "\n",
    "- $E[y] = \\Sigma_{y = 0}^n \\cdotp \\binom{n}{y} \\cdot p^y \\cdot q^{n-y}$.\n",
    "\n",
    "Step 3: Simplify the Expression\n",
    "\n",
    "Replace q with 1-p and rearranging terms.\n",
    "\n",
    "- $E[y] = \\Sigma_{y = 0}^n \\frac{n!}{y!(n-y)!} \\cdot (p)^y \\cdot (1-p)^{(n-y)}$.\n",
    "\n",
    "Step 4: Factor Out Constants\n",
    "\n",
    "Since $p$ is constant, we can  factor it out of the summation.\n",
    "\n",
    "- $E[y] = np \\, \\Sigma_{y = 0}^n \\frac{(n-1)!}{(y-1)!(n-y)!} \\cdot (p)^{(y-1)} \\cdot (1-p)^{(n-y)}$.\n",
    "\n",
    "Step 5: Rearrange the Terms\n",
    "\n",
    "- $E[y] = np \\, \\Sigma_{y = 1}^n \\frac{(n-1)!}{(y-1)!(n-y)!} \\cdot (p)^{(y-1)} \\cdot (1-p)^{(n-y)}$.\n",
    " \n",
    "Step 6: Apply the Binomial Theorem\n",
    "\n",
    "The binomial theorem states that for any positive integers n and k, one has the following equality:\n",
    "\n",
    "$(x+y)^{n}= \\Sigma_{k=0}^{n}\\binom{n}{k} x^{k} y^{n-k}$ \n",
    "\n",
    " where: $\\binom{n}{k}$ denotes the binomial coefficient.\n",
    "\n",
    "- $(p + q)^ {n -1} = \\Sigma_{k = 0}^{n-1} \\binom{n-1}{y} \\cdot (p)^{(k)} \\cdot (q)^{(n-1-k)}$\n",
    "\n",
    "By comparing the terms in th expression to the binomial theorem, we can see that:\n",
    "\n",
    "- $(p + q)^ {n-1} = \\Sigma_{y = 0}^{n} \\frac{(n-1)!}{(y)!(n-y)!} \\cdot (p)^{(y)} \\cdot (q)^{(n-y)}$\n",
    "\n",
    "Step 7: Simplify the expression\n",
    "\n",
    "The expansion of $(p + (1-p))^{n-1}$ is simply $1^{n-1}$, which equals 1. Therefore, the sum becomes 1.\n",
    "\n",
    "\n",
    "\n",
    "This simplifies to:\n",
    "\n",
    "$E[y] = np \\cdot 1$ which leads to the final simplification of $E[y] = np$.\n",
    "\n",
    "In conclusion, the expectation of a binomial distribution, $E[y] = np$, validates that the mean equals the product of the number of trials and the probability of success.\n",
    "\n",
    "**<h4>Question 3:</h4>** \n",
    "\n",
    "Probability of Recovery\n",
    "\n",
    "Given: \n",
    "\n",
    "-  Probability of success (recovery) $p = 0.30$\n",
    "-  Number of trials $n = 10$\n",
    "- Number of successes (recoveries) $y = 9$\n",
    "\n",
    "Using the binomial probability mass function:\n",
    "\n",
    "Solution: \n",
    "\n",
    "- $P(Y \\geq 9) = P(Y = 9) + P(Y = 10)$\n",
    "- $P(Y \\geq 9) = \\binom{10}{9} \\cdot (0.30)^9 \\cdot (1 - 0.30)^{10-9} + \\binom{10}{10} \\cdot (1 - 0.30)^{10-10}$\n",
    "- $P(Y \\geq 9) = 10 \\cdot (0.30)^9 \\cdot (0.70)^1 + 1 \\cdot (0.30)^{10}  \\cdot (0.70)^0$\n",
    "- $ P(Y \\geq 9) = 10 \\cdot (0.30)^9 \\cdot 0.70 + (0.30)^{10}$\n",
    "- $ P(Y \\geq 9) = 0.000137781 + 0.0000059049$\n",
    "- $ P (Y \\geq 9) \\approx 0.0001436869$ or $0.014 \\%$\n",
    "\n",
    "Hence, the probability that at least nine of ten receiving the medication will recover is $0.014 \\%$\n",
    "\n",
    "**<h4>Question 4:</h4>**\n",
    "\n",
    " Probability of Observing at Least One Defective Fuse \n",
    "Given:\n",
    "- Probability of success (a fuse being non-defective) $p = 0.95$\n",
    "- Number of trials $n = 5$\n",
    "\n",
    "Solution:\n",
    "\n",
    "- $P(At \\, least \\, one \\, defective) = 1 - P(No \\, defective)$\n",
    "- $P(At \\, least \\, one \\, defective) = 1 - P(Y = 0)$\n",
    "\n",
    "Using the binomial probability mass function:\n",
    "\n",
    "- $P(Y=0) = \\binom {5}{0} \\cdot (0.05)^0 \\cdot (1 - 0.05)^{5-0}$\n",
    "- $P(Y = 0) = (0.95)^5$\n",
    "- $P(At \\, least \\, one \\, defective) = 1 - (0.95)^5$\n",
    "- $P(At \\, least \\, one \\, defective) \\approx 1 - 0.7738$\n",
    "- $P(At \\, least \\, one \\, defective) \\approx 0.2262$\n",
    "\n",
    "Hence, the probability of observing at least one defective fuse in a sample of 5 fuses is approximately $0.2262$ or $22.62\\%$\n",
    "\n",
    "\n"
   ]
  },
  {
   "cell_type": "markdown",
   "metadata": {},
   "source": [
    "**<h3>Task 3: Consider a probility distribution of $p(y) = \\frac{\\lambda^y}{y!} e^{-\\lambda}$.</h3>**"
   ]
  },
  {
   "cell_type": "markdown",
   "metadata": {},
   "source": [
    "**<h4>Question 1:</h4>**\n",
    "\n",
    "Given probability distribution: $p(y) = \\frac{\\lambda^y}{y!} e^{-\\lambda}$\n",
    "\n",
    "Expected value formula: $E[Y] = \\Sigma_{y=0} ^ \\infty \\, y \\cdot p(y)$\n",
    "\n",
    "Step 1: Substitue the Probability Distribution into the Expected Value Formula\n",
    "\n",
    "- $E[Y] = \\Sigma_{y=0} ^ \\infty \\, y \\cdot \\frac{\\lambda^y}{y!} e^{-\\lambda}$\n",
    "\n",
    "Step 2: Factor out Constants\n",
    "\n",
    "- $E[Y] = e^{-\\lambda} \\Sigma_{y=0} ^ \\infty \\, \\frac{\\lambda^y}{(y - 1)!} $\n",
    "\n",
    "Step 3: Since $y = 0$ makes $\\frac{\\lambda^y}{(y - 1)!}$ undefined, we shift the index of summation to start from $y = 1$.\n",
    "\n",
    "- $E[Y] = e^{-\\lambda} \\Sigma_{y=1} ^ \\infty \\, \\frac{\\lambda^y}{(y - 1)!} $\n",
    "\n",
    "Step 4: Rewrite $\\frac{\\lambda^y}{(y - 1)!}$ as $\\frac{\\lambda^{(y-1)+ 1}}{(y - 1)!}$ \n",
    "\n",
    "- $E[Y] = e^{-\\lambda} \\Sigma_{y=1} ^ \\infty \\,  \\frac{\\lambda^{(y-1)+ 1}}{(y - 1)!}$\n",
    "\n",
    "Step 5: Change the index of summation to start from $y = 0$ to simplify the expression.\n",
    "\n",
    "- $E[Y] = e^{-\\lambda} \\Sigma_{y=0} ^ \\infty \\,  \\frac{\\lambda^{y+1}}{y!}$\n",
    "\n",
    "Step 6: Factor out $\\lambda$\n",
    "\n",
    "- $E[Y] = e^{-\\lambda} \\lambda \\Sigma_{y=0} ^ \\infty \\, \\frac {\\lambda^{y}}{y!}$\n",
    "\n",
    "Step 7: Recall that $e^{\\lambda} =  \\Sigma_{y=0} ^ \\infty \\, \\frac {\\lambda^{y}}{y!}$\n",
    "\n",
    "-  $E[Y] = e^{-\\lambda} \\lambda e^{\\lambda} $\n",
    "\n",
    "Step 8: Simplify: \n",
    "\n",
    "-  $E[Y] =  \\lambda$\n",
    "\n",
    "To conclude, the general formula for the expected value of the given distribution is $E[Y] =  \\lambda$\n"
   ]
  },
  {
   "cell_type": "markdown",
   "metadata": {},
   "source": [
    "\n",
    "**<h4>Question 2:</h4>**\n",
    "\n",
    "Given:\n",
    "- $\\lambda = 5$\n",
    "\n",
    "Asked:\n",
    "- Find the probability that none of the regions will contain seedlings, i.e., $ P(Y = 0)$ where $Y$ follows a Poisson distribution with parameter $\\lambda = 5$ .\n",
    "\n",
    "Using the formula for the Poisson distribution:\n",
    "\n",
    "- $P(Y = y) = \\frac{\\lambda^y}{y!} e^{-\\lambda}$\n",
    "\n",
    "For $y = 0$:\n",
    "\n",
    "$ P(Y = 0) = \\frac{5^0}{0!} e^{-5} $\n",
    "\n",
    "$ = e^{-5} $\n",
    "\n",
    "Calculating this probability:\n",
    "\n",
    "$P(Y = 0) \\approx e^{-5} $\n",
    "\n",
    "$\\approx 0.006737947$\n",
    "\n",
    "Futhermore, the probability that none of the regions will contain seedlings is approximately $ 0.0067$ or $ 0.67\\%$."
   ]
  }
 ],
 "metadata": {
  "kernelspec": {
   "display_name": "base",
   "language": "python",
   "name": "python3"
  },
  "language_info": {
   "codemirror_mode": {
    "name": "ipython",
    "version": 3
   },
   "file_extension": ".py",
   "mimetype": "text/x-python",
   "name": "python",
   "nbconvert_exporter": "python",
   "pygments_lexer": "ipython3",
   "version": "3.11.7"
  }
 },
 "nbformat": 4,
 "nbformat_minor": 2
}
